LeanApi.lean
@@ -17,4 +17,5 @@ import LeanApi.Http.Features
 import LeanApi.Http.Multipart
 import LeanApi.Http.Typed
 import LeanApi.Http.Endpoint
+import LeanApi.Http.DbEndpoint
 import LeanApi.Props
